
\chapter{Завдання \theHchapter}

\begin{tcolorbox}[title=Завдання]
    Нехай $x \in [0, 1], n \in N$. Доведiть тотожнiсть
    $$ \sum\limits_{k=0}^{n}(\frac{k}{n} - x)^2 C_n^kx^k(1-x)^{n-k}=
    \frac{x(1-x)}{n} $$
\end{tcolorbox}

\center{\bfseries Розв'язання:}


Біном Ньютона


$ 1^n = (1 - x + x)^n = \sum\limits_{k=0}^{n}C_n^kx^k(1 - x)^{n - k} $


Позначимо за $f(x) = \sum\limits_{k=0}^{n}C_n^kx^k(1 - x)^{n - k} = 1$


Тоді $\frac{df(x)}{dx} = 
\sum\limits_{k=0}^{n}kC_n^kx^{k-1}(1 - x)^{n - k} - 
\sum\limits_{k=0}^{n}(n - k)C_n^kx^k(1 - x)^{n - k - 1} = 0$


$ 
\sum\limits_{k=0}^{n}kC_n^kx^{k-1}(1 - x)^{n - k - 1} -
\cancel{\sum\limits_{k=0}^{n}kC_n^kx^{k}(1 - x)^{n - k - 1}} -$


$-\sum\limits_{k=0}^{n}nC_n^kx^k(1 - x)^{n - k - 1} + 
\cancel{\sum\limits_{k=0}^{n}kC_n^kx^k(1 - x)^{n - k - 1}} = 0$


$
\sum\limits_{k=0}^{n}kC_n^kx^{k-1}(1 - x)^{n - k - 1} -
\sum\limits_{k=0}^{n}nC_n^kx^k(1 - x)^{n - k - 1} = 0$ 


$\sum\limits_{k=0}^{n}(k - nx)C_n^kx^{k-1}(1 - x)^{n - k - 1} = 0  $



$\sum\limits_{k=0}^{n}\frac{k}{n}
C_n^kx^{k}(1 - x)^{n - k} =  
\sum\limits_{k=0}^{n}x
C_n^kx^{k}(1 - x)^{n - k} =
x$


\newpage
$\frac{d^2f(x)}{dx^2} = 
\sum\limits_{k=0}^{n}C_n^kx^{k - 2}(1 - x)^{(n - k -2)}(
    k(k - 1)(1 - x)^2 - 2 k (n - k) x (1 - x) +
    (n - k)(n - k - 1) x^2)=$


$
=\sum\limits_{k=0}^{n}C_n^kx^{k - 2}(1 - x)^{(n - k -2)}(
    k^2 - k - \cancel{2xk^2} + 2xk + \cancel{x^2k^2} - \cancel{kx^2} -
    2knx + \cancel{2knx^2} + \cancel{2k^2x} - \cancel{2k^2x^2} +
    n^2x^2 - \cancel{nkx^2} - nx^2 - \cancel{knx^2} + 
    \cancel{k^2x^2} + \cancel{kx^2}
)=
$


$
=\sum\limits_{k=0}^{n}C_n^kx^{k - 2}(1 - x)^{(n - k -2)}(
    k^2 - k + 2kx - 2knx - 2 k^2 x^2 + n^2x^2 - nx^2
)
$


$
\sum\limits_{k=0}^{n}C_n^kx^{k - 2}(1 - x)^{(n - k -2)}k^2=
nx -2nx^2 +2 n^2x^2 - n^2x^2 + nx^2
$



$
\frac{1}{n}\sum\limits_{k=0}^{n}C_n^kx^{k - 2}(1 - x)^{(n - k -2)}k^2=
x - x^2 + nx^2
$


\newpage

$ \sum\limits_{k=0}^{n}(\frac{k}{n} - x)^2 C_n^kx^k(1-x)^{n-k} = 
\sum\limits_{k=0}^{n}\frac{k}{n}(\frac{k}{n} - x) C_n^kx^k(1-x)^{n-k} - 
x\underbrace{\sum\limits_{k=0}^{n}(\frac{k}{n} - x) C_n^kx^k(1-x)^{n-k}}_{\mbox{0}} = $


$=\frac{1}{n}\sum\limits_{k=0}^{n}k(\frac{k}{n} - x) C_n^kx^k(1-x)^{n-k} = 
\frac{1}{n}(\sum\limits_{k=0}^{n}\frac{k^2}{n} C_n^kx^k(1-x)^{n-k} - 
\sum\limits_{k=0}^{n}kxC_n^kx^k(1-x)^{n-k})=$


$=\frac{1}{n}\sum\limits_{k=0}^{n}\frac{k^2}{n} C_n^kx^k(1-x)^{n-k} - 
x^2 = \frac{x - x^2 +nx^2}{n} - x^2 =\frac{x - x^2}{n}$


Доведено!
