
\section{задача}


\begin{tcolorbox}[title = Умова]
    Нехай $g : E \rightarrow \mathbb{R} \cup {+\infty}$ — власна замкнена 
    та опукла функцiя. Доведiть, що
    $$(prox_g(x) - prox_g(y), x - y) \geq \|prox_g(x) -  prox_g(y)\|_2^2 \quad 
    \forall x, y \in E$$
\end{tcolorbox}

З задачі 2 випливає, що при $z_1 = prox_g(y), z_2 = prox_g(x)$
$$ g(p) - g(prox_g(y)) \geq (y -prox_g(y), p - prox_g(y)) = 
(y - prox_g(y), p) - (y - prox_g(y), prox_g(y))$$
$$ g(p) - g(prox_g(x)) \geq (x -prox_g(x), p - prox_g(x)) = 
(x - prox_g(x), p) - (x - prox_g(x), prox_g(x))$$

Виберемо $p = prox_g(x)$ і $p = prox_g(y)$ відповідно. Отримаємо

$$ g(prox_g(x)) - g(prox_g(y)) \geq 
(y - prox_g(y), prox_g(x)) - (y - prox_g(y), prox_g(y))$$
$$ g(prox_g(y)) - g(prox_g(x)) \geq 
(x - prox_g(x), prox_g(y)) - (x - prox_g(x), prox_g(x))$$

Додамо нерівності 

$$ 
(y - prox_g(y), prox_g(x)) - (y - prox_g(y), prox_g(y)) +
(x - prox_g(x), prox_g(y)) - (x - prox_g(x), prox_g(x)) \le 0
$$

$$
(y, prox_g(x)) - (prox_g(y), prox_g(x)) - (y, prox_g(y)) +$$
$$+(x, prox_g(y)) - (prox_g(x), prox_g(y)) - (x, prox_g(x)) + \|prox_g(x) - prox_g(y)\|^2 \le 0
$$
$$(prox_g(y) - prox_g(x), x - y) + \|prox_g(x) - prox_g(y)\|^2 \le 0 $$

Доведено